src/coq/Analysis/Kildall.v
@@ -225,10 +225,11 @@ Module ForwardSolver (PC:UsualDecidableType) (LAT:LATTICE)<:
     induction bs as [|b']. contradiction.
     simpl; intros. destruct H0. subst b'.
     set (a' := fold_left _ _ _). pattern a'.
-  (*   eapply fold_left_1; eauto.  *)
-  (*   apply IHbs. assumption. *)
-  (* Qed. *)
-  Admitted.
+    eapply fold_left_1; eauto.
+    subst; reflexivity.
+    apply IHbs; assumption.
+  Qed.
+  
 
   Lemma prop_n_out : forall o ns s s' n,
     s' = fold_left (prop_succ o) ns s ->
