src/coq/Handlers/MemoryTheory.v
@@ -1,3 +1,4 @@
+(* begin hide *)
 From Coq Require Import
      Morphisms ZArith List String Lia
      FSets.FMapAVL
@@ -2991,41 +2992,6 @@ Section Memory_Stack_Theory.
       unfold no_overlap_dtyp.
       unfold no_overlap.
       left. auto.
-    Qed.
-
-    Lemma read_in_mem_block_type :
-      forall bytes a τ v,
-        is_supported τ ->
-        read_in_mem_block bytes a τ = v ->
-        uvalue_has_dtyp v τ.
-    Proof.
-      intros bytes a τ v SUP READ.
-
-      unfold read_in_mem_block in READ.
-      unfold deserialize_sbytes in READ.
-      break_match_hyp.
-      2: {
-        (* If any byte is undef, then we get a UVALUE_Undef of the appropriate type *)
-        subst.
-        constructor.
-      }
-
-      (* Issue with pointers deserializing to None... *)
-    Admitted.
-
-    Lemma read_type :
-      forall m p τ v,
-        is_supported τ ->
-        read m p τ = inr v ->
-        uvalue_has_dtyp v τ.
-    Proof.
-      intros m p τ v SUP READ.
-      unfold read in *.
-      break_match; inversion READ.
-      clear H0.
-      break_match; subst.
-      inversion READ.
-      eapply read_in_mem_block_type; eauto.
     Qed.
 
 End Memory_Stack_Theory.
